Reorganized element-list abstraction

model/BTrees.v
@@ -778,4 +778,187 @@ Proof.
   - apply bf_final. apply bf_val. apply bf_nil.
 Qed.
 
+(** Abstraction of cursors as bi-directional list of key-value pairs
+  * Proofs about this abstraction and the implementation
+  *)
+
+Fixpoint elements' (f : treelist) (base: list (key * V)) : list (key * V) :=
+  match f with
+  | tl_cons (node k f1) f2 => elements' f1 (elements' f2 base)
+  | tl_cons (final f1) f2 => elements' f1 (elements' f2 base)
+  | tl_cons (val k v) f2 => (k,v)::(elements' f2 base)
+  | tl_nil => base
+  end.
+
+Fixpoint elements (f : treelist) : list (key * V) := elements' f [].
+
+Fixpoint right_el (f : treelist) (base : list (key * V)) : list (key * V) :=
+  match f with
+  | tl_cons (node k f1) f2 => right_el f2 (right_el f1 base)
+  | tl_cons (final f1) f2 => right_el f2 (right_el f1 base)
+  | tl_cons (val k v) f2 => right_el f2 (base++[(k,v)])
+  | tl_nil => base
+  end.
+
+Fixpoint left_el (f : treelist) (base : list (key * V)) : list (key * V) :=
+  match f with
+  | tl_cons (node k f1) f2 => left_el f1 (left_el f2 base)
+  | tl_cons (final f1) f2 => left_el f1 (left_el f2 base)
+  | tl_cons (val k v) f2 => (left_el f2 base) ++ [(k,v)]
+  | tl_nil => base
+  end.
+
+Fixpoint cursor_elements' (cn : list nat) (cf : list treelist) (left : list (key * V)) (right : list (key * V))
+  : (list (key * V)) * (list (key * V)) :=
+  match (cn,cf) with
+  | (n::cn,f::cf) =>
+    (match point n f with (f1,f2) => cursor_elements' cn cf (left_el f1 left) (right_el f2 right) end)
+  | (_,_) => (left,right)
+  end.
+
+Definition cursor_elements (c : cursor) : list (key * V) * list (key * V) :=
+  match c with
+  | (n::cn,f::cf) =>
+    (match point_first n f with (f1,f2) => cursor_elements' cn cf (left_el f1 []) (right_el f2 []) end)
+  | (_,_) => ([],[])
+  end.
+
+(* Cursor to list of elements : cons in both directions *)
+(* get returns the next thing in that list! *)
+
+Definition right_el_P (t : tree) : Prop := forall k f b,
+  t = node k f \/ t = final f ->
+  exists l', right_el f b = b++l'.
+
+Theorem right_el_interior : forall f b,
+  exists l', right_el f b = b++l'.
+Proof.
+  induction f using treelist_tree_rec with (P := right_el_P).
+  - unfold right_el_P. intros. inversion H; inversion H0. subst. apply IHf.
+  - unfold right_el_P. intros. inversion H; inversion H0. subst. apply IHf.
+  - unfold right_el_P. intros. inversion H; inversion H0.
+  - intros. unfold right_el. exists []. rewrite app_nil_r. reflexivity.
+  - intros. destruct t eqn:e.
+    + simpl. unfold right_el_P in IHf.
+      assert (exists l', right_el t0 b0 = b0++l').
+      { apply IHf with k. left. reflexivity. }
+      inversion H. rewrite H0. destruct IHf0 with (b0 ++ x).
+      exists (x++x0). rewrite H1. rewrite app_assoc. reflexivity.
+    + simpl. unfold right_el_P in IHf.
+      assert (exists l', right_el t0 b0 = b0++l').
+      { apply IHf with zero. right. reflexivity. }
+      inversion H. rewrite H0. destruct IHf0 with (b0 ++ x).
+      exists (x ++ x0). rewrite H1. rewrite app_assoc. reflexivity.
+    + simpl. destruct IHf0 with (b0 ++ [(k,v)]).
+      exists ((k,v)::x). rewrite H. rewrite <- app_assoc. reflexivity.
+Qed.
+
+Definition left_el_P (t : tree) : Prop := forall k f b,
+  t = node k f \/ t = final f ->
+  exists l', left_el f b = b++l'.
+
+Theorem left_el_interior : forall f b,
+  exists l', left_el f b = b++l'.
+Proof.
+  induction f using treelist_tree_rec with (P := left_el_P).
+  - unfold left_el_P. intros. inversion H; inversion H0. subst. apply IHf.
+  - unfold left_el_P. intros. inversion H; inversion H0. subst. apply IHf.
+  - unfold left_el_P. intros. inversion H; inversion H0.
+  - intros. unfold left_el. exists []. rewrite app_nil_r. reflexivity.
+  - intros. destruct t eqn:e.
+    + simpl. unfold left_el_P in IHf.
+      assert (exists l', left_el f b0 = b0++l'). { apply IHf0. }
+      inversion H. rewrite H0. destruct IHf with k t0 (b0 ++ x).
+      * left. reflexivity.
+      * exists (x ++ x0). rewrite H1. rewrite app_assoc. reflexivity.
+    + simpl. unfold left_el_P in IHf.
+      assert (exists l', left_el f b0 = b0++l'). { apply IHf0. }
+      inversion H. rewrite H0. destruct IHf with zero t0 (b0 ++ x).
+      * right. reflexivity.
+      * exists (x ++ x0). rewrite H1. rewrite app_assoc. reflexivity.
+    + simpl. destruct IHf0 with b0. rewrite H.
+      exists (x++[(k,v)]). rewrite <- app_assoc. reflexivity.
+Qed.
+
+Theorem bases_interior : forall cn cf left right,
+  exists l' r', cursor_elements' cn cf left right = (left++l',right++r').
+Proof.
+  induction cn,cf.
+  - intros. simpl. exists [], []. repeat rewrite app_nil_r. reflexivity.
+  - intros. simpl. exists [], []. repeat rewrite app_nil_r. reflexivity.
+  - intros. simpl. exists [], []. repeat rewrite app_nil_r. reflexivity.
+  - intros. simpl. destruct (point a t).
+    destruct IHcn with cf (left_el t0 left) (right_el t1 right). destruct H. rewrite H.
+    assert (exists l', left_el t0 left = left++l'). { apply left_el_interior. }
+    assert (exists r', right_el t1 right = right++r'). { apply right_el_interior. }
+    inversion H0. inversion H1. rewrite H2. rewrite H3.
+    exists (x1++x), (x2++x0). repeat rewrite app_assoc. reflexivity.
+Qed.
+
+Theorem cursor_elements'_rec : forall cn cf n f l r l' r',
+  (n >= treelist_length f) ->
+  cursor_elements' cn cf (left_el f l) r = (l',r') ->
+  exists l'', cursor_elements' (n::cn) (f::cf) l r = (l'',r').
+Proof.
+  induction cn,cf; intros; apply point_treelist_length in H;
+  simpl in H0; simpl; rewrite H; simpl; exists l'; apply H0.
+Qed.
+
+Theorem cursor_elements'_sides_indep : forall cn cf l1 l2 l' r r',
+  cursor_elements' cn cf l1 r = (l',r') ->
+  exists l'', cursor_elements' cn cf l2 r = (l'',r').
+Proof.
+  induction cn,cf; intros.
+  - simpl in H. simpl. inversion H. subst. exists l2. reflexivity.
+  - simpl in H. simpl. inversion H. subst. exists l2. reflexivity.
+  - simpl in H. simpl. inversion H. subst. exists l2. reflexivity.
+  - simpl in H. simpl. destruct (point a t).
+    apply IHcn with (left_el t0 l1) l'. apply H.
+Qed.
+
+Theorem cursor_elements'_next_node : forall cn cf n f cn' cf' l1 l2 l' r r',
+  n >= treelist_length f ->
+  next_node (n::cn) (f::cf) = (cn',cf') ->
+  cursor_elements' (n::cn) (f::cf) l1 r = (l',r') ->
+  exists l'', cursor_elements' cn' cf' l2 r = (l'',r').
+Proof.
+  induction cn,cf; intros.
+  - simpl in H0. simpl in H1. destruct (point n f) eqn:e. destruct t0; try (destruct t0).
+    + inversion H0. subst. simpl in H1. simpl. rewrite e.
+      simpl. inversion H1. exists (left_el t l2). reflexivity.
+    + inversion H0. subst. simpl in H1. unfold cursor_elements'.
+
+  - apply point_treelist_length in H. simpl in H0.
+    rewrite H in H0. inversion H0. subst. simpl.
+
+
+
+ simpl in H0. inversion H. subst. reflexivity.
+  - simpl in H. inversion H. subst. reflexivity.
+  - simpl in H. inversion H. subst. reflexivity.
+  - simpl. destruct (point n t) eqn:e1. destruct t1.
+    + admit.
+    + simpl in H. rewrite e1 in H. destruct t1.
+      * inversion H. simpl.
+
+(* Needs the addition of some assumption about the structure of c *)
+(* Will rely on a lemma about get_next within get_tree -- but what? *)
+Theorem get_cursor_elements : forall c l1 l2 k v,
+  cursor_elements c = (l1,(k,v)::l2) -> get_tree c = Some (val k v).
+Proof.
+  destruct c as [cn cf]. induction cn,cf; simpl; intros.
+  - inversion H.
+  - inversion H.
+  - inversion H.
+  - destruct (point_first a t) eqn:e2.
+    assert (exists l' r', cursor_elements' cn cf (left_el t0 []) (right_el t1 []) = ((left_el t0 [])++l', (right_el t1 [])++r')).
+    { apply bases_interior. }
+    inversion H0. inversion H1.
+    destruct (right_el t1 []) eqn:e3.
+    + admit.
+    + rewrite H2 in H. inversion H. subst. destruct t1.
+      * inversion e3.
+      * simpl in e3. destruct t1. admit. admit. admit.
+Admitted.
+
 End BTREES.
